Stratproof (#45)
* wip

* more qeds

* finish proof

* opam fix

* ci fix

* opam fix

theory/Util/IntHash.v
@@ -23,3 +23,21 @@ Proof.
     rewrite eqb_false_spec in Heq.
     apply Heq; congruence.
 Defined.
+
+Class CondIntHash {X : Type} (P : X -> Prop) : Type := {
+  chash : X -> int;
+  chash_inj : forall x x', P x -> P x' -> chash x = chash x' -> x = x'
+  }.
+
+Definition CondIntHash_dec {X} {P : X -> Prop} `{CondIntHash X P} : forall x x' : X,
+  P x -> P x' ->
+  {x = x'} + {x <> x'}.
+Proof.
+  intros.
+  destruct (eqb (chash x) (chash x')) eqn:Heq.
+  - rewrite eqb_spec in Heq.
+    left; now apply chash_inj.
+  - right; intro.
+    rewrite eqb_false_spec in Heq.
+    apply Heq; congruence.
+Defined.
